semantics: interpret UB last
This is the proper thing to do since in the future we want dialect
handlers to be able to emit UB. It's also helpful in proofs since we
don't have to sift SSA events through interpUB' at the first layer.

Amazingly, this commit is accompanied by a full refresh of the proofs
in ArithSemantics.lean, with only minor encounters of the WF induction
bug.

Ultimately simp_itree remains more efficient in development effort
than all the ops.*.sem theorems, which just re-state what we've already
written. It would be nice to get rid of these lemmas, either with
simp_itree, or with some conv + unfolding the ArithE handler.

MLIR/Dialects/ArithSemantics.lean
@@ -227,6 +227,15 @@ private abbrev ops.negi (output input: SSAVal): BasicBlockStmt arith :=
   .StmtAssign output none <|
     .mk "negi" [input] [] [] (.mk []) (.fn (.tuple [.i32]) .i32)
 
+private abbrev ops.zext (sz₁ sz₂: Nat) (output input: SSAVal): BasicBlockStmt arith :=
+  .StmtAssign output none <|
+    .mk "zext" [input] [] [] (.mk [])
+      (.fn (.tuple [.int .Signless sz₁]) (.int .Signless sz₂))
+
+private abbrev ops.select (output cond t f: SSAVal): BasicBlockStmt arith :=
+  .StmtAssign output none <|
+    .mk "select" [cond, t, f] [] [] (.mk []) (.fn (.tuple [.i1, .i32, .i32]) .i32)
+
 private abbrev ops._binary (name: String) (output lhs rhs: SSAVal):
     BasicBlockStmt arith :=
   .StmtAssign output none <|
@@ -240,8 +249,8 @@ private abbrev ops.xori := ops._binary "xori"
 
 private theorem ops.constant.sem output value:
     denoteBBStmt arith (ops.constant output value) =
-  Fitree.Vis (E := UBE +' SSAEnvE arith +' Semantics.E arith)
-    (Sum.inr <| Sum.inl <| SSAEnvE.Set .i32 output (FinInt.ofInt 32 value)) fun _ =>
+  Fitree.Vis (E := SSAEnvE arith +' Semantics.E arith +' UBE)
+    (Sum.inl <| SSAEnvE.Set .i32 output (FinInt.ofInt 32 value)) fun _ =>
   Fitree.ret (BlockResult.Next (δ := arith)
     ⟨.i32, FinInt.ofInt 32 value⟩) := by
   simp [ops.constant, denoteBBStmt, denoteOp, Semantics.semantics_op]
@@ -250,12 +259,36 @@ private theorem ops.constant.sem output value:
 
 private theorem ops.negi.sem output input:
     denoteBBStmt arith (ops.negi output input) =
-  Fitree.Vis (E := UBE +' SSAEnvE arith +' Semantics.E arith)
-    (Sum.inr <| Sum.inl <| SSAEnvE.Get .i32 input) fun r =>
-  Fitree.Vis (Sum.inr <| Sum.inr <| ArithE.NegI 32 r) fun r =>
-  Fitree.Vis (Sum.inr <| Sum.inl <| SSAEnvE.Set .i32 output r) fun _ =>
+  Fitree.Vis (E := SSAEnvE arith +' Semantics.E arith +' UBE)
+    (Sum.inl <| SSAEnvE.Get .i32 input) fun r =>
+  Fitree.Vis (Sum.inr <| Sum.inl <| ArithE.NegI 32 r) fun r =>
+  Fitree.Vis (Sum.inl <| SSAEnvE.Set .i32 output r) fun _ =>
   Fitree.ret (BlockResult.Next ⟨.i32, r⟩) := by
   simp [ops.negi, denoteBBStmt, denoteOp, Semantics.semantics_op]
+  simp_itree
+
+private theorem ops.zext.sem sz₁ sz₂ output input:
+    denoteBBStmt arith (ops.zext sz₁ sz₂ output input) =
+  Fitree.Vis (E := SSAEnvE arith +' Semantics.E arith +' UBE)
+    (Sum.inl <| @SSAEnvE.Get _ _ _ _ (.int .Signless sz₁) (instInhabitedEval _) input) fun r =>
+  Fitree.Vis (Sum.inr <| Sum.inl <| ArithE.Zext sz₁ sz₂ r) fun r =>
+  Fitree.Vis (Sum.inl <| SSAEnvE.Set (.int .Signless sz₂) output r) fun _ =>
+  Fitree.ret (BlockResult.Next ⟨.int .Signless sz₂, r⟩) := by
+  simp [ops.zext, denoteBBStmt, denoteOp, Semantics.semantics_op]
+  simp_itree
+
+private theorem ops.select.sem output cond t f:
+    denoteBBStmt arith (ops.select output cond t f) =
+  Fitree.Vis (E := SSAEnvE arith +' Semantics.E arith +' UBE)
+    (Sum.inl <| SSAEnvE.Get .i1 cond) fun cond =>
+  Fitree.Vis (E := SSAEnvE arith +' Semantics.E arith +' UBE)
+    (Sum.inl <| SSAEnvE.Get .i32 t) fun t =>
+  Fitree.Vis (E := SSAEnvE arith +' Semantics.E arith +' UBE)
+    (Sum.inl <| SSAEnvE.Get .i32 f) fun f =>
+  Fitree.Vis (Sum.inr <| Sum.inl <| ArithE.Select 32 cond t f) fun r =>
+  Fitree.Vis (Sum.inl <| SSAEnvE.Set .i32 output r) fun _ =>
+  Fitree.ret (BlockResult.Next ⟨.i32, r⟩) := by
+  simp [ops.select, denoteBBStmt, denoteOp, Semantics.semantics_op]
   simp_itree
 
 private theorem ops._binary.sem name ctor output lhs rhs:
@@ -264,11 +297,11 @@ private theorem ops._binary.sem name ctor output lhs rhs:
         (IOp.mk name [⟨.i32, n⟩, ⟨.i32, m⟩] [] 0 (.mk []) (.fn (.tuple [.i32, .i32]) .i32)) =
       binary_semantics_op name [⟨.i32, n⟩, ⟨.i32, m⟩] ctor) →
     denoteBBStmt arith (ops._binary name output lhs rhs) =
-  Fitree.Vis (E := UBE +' SSAEnvE arith +' Semantics.E arith)
-    (Sum.inr <| Sum.inl <| SSAEnvE.Get .i32 lhs) fun lhs =>
-  Fitree.Vis (Sum.inr <| Sum.inl <| SSAEnvE.Get .i32 rhs) fun rhs =>
-  Fitree.Vis (Sum.inr <| Sum.inr <| ctor 32 lhs rhs) fun r =>
-  Fitree.Vis (Sum.inr <| Sum.inl <| SSAEnvE.Set .i32 output r) fun _ =>
+  Fitree.Vis (E := SSAEnvE arith +' Semantics.E arith +' UBE)
+    (Sum.inl <| SSAEnvE.Get .i32 lhs) fun lhs =>
+  Fitree.Vis (Sum.inl <| SSAEnvE.Get .i32 rhs) fun rhs =>
+  Fitree.Vis (Sum.inr <| Sum.inl <| ctor 32 lhs rhs) fun r =>
+  Fitree.Vis (Sum.inl <| SSAEnvE.Set .i32 output r) fun _ =>
   Fitree.ret (BlockResult.Next ⟨.i32, r⟩) := by
   intro h
   simp [denoteBBStmt, denoteOp, Semantics.semantics_op]
@@ -325,9 +358,7 @@ theorem equivalent (n m: FinInt 32):
   simp [LHS, RHS, run, Semantics.handle]
   rw [ops.addi.sem]
   rw [ops.addi.sem]
-  simp
-  simp [interpSSA', SSAEnvE.handle, SSAEnv.get, SSAEnv.set, cast_eq]
-  simp [Fitree.interp_bind]
+  simp [SSAEnvE.handle, cast_eq]
   -- Unfold ArithE.handle only where it is applied to an explicit effect
   repeat conv in ArithE.handle _ _ => simp [ArithE.handle]
   simp [FinInt.add_comm]
@@ -360,16 +391,13 @@ def INPUT (C X C2: FinInt 32): SSAEnv arith := SSAEnv.One [
 ]
 
 theorem equivalent (C X C2: FinInt 32):
-    (run ⟦LHS⟧ (INPUT C X C2) |>.snd.get "r" .i32) =
-    (run ⟦RHS⟧ (INPUT C X C2) |>.snd.get "r" .i32) := by
+    semanticPostCondition₂
+      (run ⟦LHS⟧ (INPUT C X C2))
+      (run ⟦RHS⟧ (INPUT C X C2))
+    fun _ env₁ _ env₂ =>
+      env₁.get "r" .i32 = env₂.get "r" .i32 := by
   simp [LHS, RHS, INPUT]
   simp [run, denoteBB, denoteBBStmts, denoteBBStmt, denoteOp]; simp_itree
-  simp [interpUB']; simp_itree
-  simp [interpSSA', Fitree.interpState, SSAEnvE.handle, SSAEnv.get]; simp_itree
-  simp [SSAEnv.get]; simp_itree
-  simp [SSAEnv.get]; simp_itree
-  simp [SSAEnv.get]; simp_itree
-  simp [SSAEnv.get]; simp_itree
   apply FinInt.sub_add_dist
 
 /-
@@ -434,8 +462,14 @@ def INPUT (C X: FinInt 32): SSAEnv arith := SSAEnv.One [
 ]
 
 theorem equivalent (C X: FinInt 32):
-    (run ⟦LHS⟧ (INPUT C X) |>.snd.get "r" .i32) =
-    (run ⟦RHS⟧ (INPUT C X) |>.snd.get "r" .i32) := by
+  semanticPostCondition₂
+    (run ⟦LHS⟧ (INPUT C X))
+    (run ⟦RHS⟧ (INPUT C X))
+  fun _ env₁ _ env₂ =>
+    env₁.get "r" .i32 = env₂.get "r" .i32 := by
+  -- TODO: If we could simplify `denoteTypedArgs` we could save a lot of work
+  -- TODO: here. But it triggers the WF-induction bug, so we instead we unfold
+  -- TODO: the SSA stuff later. Investigate.
   simp [INPUT, LHS, RHS, run, denoteBBStmts, denoteBB]
   rw [ops.constant.sem]
   rw [ops.negi.sem]
@@ -444,9 +478,7 @@ theorem equivalent (C X: FinInt 32):
   rw [ops.constant.sem]
   rw [ops.subi.sem]
   rw [ops.subi.sem]
-  simp [interpUB']; dsimp_itree
-  simp [interpSSA', Fitree.interpState, SSAEnvE.handle]; dsimp_itree
-  repeat (simp [SSAEnv.get, SSAEnv.set]; dsimp_itree)
+  simp [interpSSA', Fitree.interpState, SSAEnvE.handle]; simp_itree
   apply FinInt.comp_add (by decide)
 end th3
 
@@ -477,18 +509,14 @@ def INPUT (A B: FinInt 32): SSAEnv arith := SSAEnv.One [
 ]
 
 theorem equivalent (A B: FinInt 32):
-    (run ⟦LHS⟧ (INPUT A B) |>.snd.get "r" .i32) =
-    (run ⟦RHS⟧ (INPUT A B) |>.snd.get "r" .i32) := by
+  semanticPostCondition₂
+    (run ⟦LHS⟧ (INPUT A B))
+    (run ⟦RHS⟧ (INPUT A B))
+  fun _ env₁ _ env₂ =>
+    env₁.get "r" .i32 = env₂.get "r" .i32 := by
   simp [LHS, RHS, INPUT]
   simp [run, denoteBB, denoteBBStmts, denoteBBStmt, denoteOp]; simp_itree
-  simp [interpUB']; simp_itree
-  simp [interpSSA', Fitree.interpState, SSAEnvE.handle, SSAEnv.get]; simp_itree
-  simp [SSAEnv.get]; simp_itree
-  simp [SSAEnv.get]; simp_itree
-  simp [SSAEnv.get]; simp_itree
-  simp [SSAEnv.get]; simp_itree
-  apply Eq.symm
-  apply FinInt.neg_add_dist
+  rw [FinInt.neg_add_dist]
 end th4
 
 /- LLVM InstCombine: `-(X - Y) --> (Y - X)`
@@ -516,15 +544,13 @@ def INPUT (X Y: FinInt 32): SSAEnv arith := SSAEnv.One [
 ]
 
 theorem equivalent (X Y: FinInt 32):
-    (run ⟦LHS⟧ (INPUT X Y) |>.snd.get "r" .i32) =
-    (run ⟦RHS⟧ (INPUT X Y) |>.snd.get "r" .i32) := by
+  semanticPostCondition₂
+    (run ⟦LHS⟧ (INPUT X Y))
+    (run ⟦RHS⟧ (INPUT X Y))
+  fun _ env₁ _ env₂ =>
+    env₁.get "r" .i32 = env₂.get "r" .i32 := by
   simp [LHS, RHS, INPUT]
   simp [run, denoteBB, denoteBBStmts, denoteBBStmt, denoteOp]; simp_itree
-  simp [interpUB']; simp_itree
-  simp [interpSSA', Fitree.interpState, SSAEnvE.handle, SSAEnv.get]; simp_itree
-  simp [SSAEnv.get]; simp_itree
-  simp [SSAEnv.get]; simp_itree
-  simp [SSAEnv.get]; simp_itree
   apply FinInt.neg_sub_dist
 end th5
 
@@ -564,8 +590,11 @@ def INPUT (A B: FinInt 32): SSAEnv arith := SSAEnv.One [
 ]
 
 theorem equivalent (A B: FinInt 32):
-    (run ⟦LHS⟧ (INPUT A B) |>.snd.get "r" .i32) =
-    (run ⟦RHS⟧ (INPUT A B) |>.snd.get "r" .i32) := by
+  semanticPostCondition₂
+    (run ⟦LHS⟧ (INPUT A B))
+    (run ⟦RHS⟧ (INPUT A B))
+  fun _ env₁ _ env₂ =>
+    env₁.get "r" .i32 = env₂.get "r" .i32 := by
   simp [INPUT, LHS, RHS, run, denoteBBStmts, denoteBB]
   rw [ops.constant.sem]
   rw [ops.addi.sem]
@@ -573,9 +602,7 @@ theorem equivalent (A B: FinInt 32):
   rw [ops.xori.sem]
   rw [ops.addi.sem]
   rw [ops.subi.sem]
-  simp [interpUB']; dsimp_itree
-  simp [interpSSA', Fitree.interpState, SSAEnvE.handle]; dsimp_itree
-  repeat (simp [SSAEnv.get, SSAEnv.set]; dsimp_itree)
+  simp [interpSSA', Fitree.interpState, SSAEnvE.handle]; simp_itree
   apply FinInt.plus_one_plus_comp
 end th6
 
@@ -615,8 +642,11 @@ def INPUT (X Y: FinInt 32): SSAEnv arith := SSAEnv.One [
 ]
 
 theorem equivalent (X Y: FinInt 32):
-    (run ⟦LHS⟧ (INPUT X Y) |>.snd.get "r" .i32) =
-    (run ⟦RHS⟧ (INPUT X Y) |>.snd.get "r" .i32) := by
+  semanticPostCondition₂
+    (run ⟦LHS⟧ (INPUT X Y))
+    (run ⟦RHS⟧ (INPUT X Y))
+  fun _ env₁ _ env₂ =>
+    env₁.get "r" .i32 = env₂.get "r" .i32 := by
   simp [INPUT, LHS, RHS, run, denoteBB, denoteBBStmts]
   rw [ops.constant.sem]
   rw [ops.negi.sem]
@@ -624,9 +654,7 @@ theorem equivalent (X Y: FinInt 32):
   rw [ops.xori.sem]
   rw [ops.subi.sem]
   rw [ops.subi.sem]
-  simp [interpUB']; dsimp_itree
-  simp [interpSSA', Fitree.interpState, SSAEnvE.handle]; dsimp_itree
-  repeat (simp [SSAEnv.get, SSAEnv.set]; dsimp_itree)
+  simp [interpSSA', Fitree.interpState, SSAEnvE.handle]; simp_itree
   apply FinInt.comp_sub_comp
 end th7
 
@@ -642,7 +670,8 @@ theorem FinInt.addfull_xor_and (A B: FinInt sz):
     | next bA A', next bB B' =>
       simp [HXor.hXor, HAnd.hAnd, HOr.hOr, xor, and, or, logic2] at *
       simp [addfull, ih]
-      cases bA <;> cases bB <;> decide
+      cases bA <;> cases bB <;> decide  repeat (simp [SSAEnv.get, SSAEnv.set]; dsimp_itree)
+
 
 theorem FinInt.add_xor_and (A B: FinInt sz):
     (A ^^^ B) + (A &&& B) = (A ||| B) := by
@@ -664,13 +693,13 @@ def INPUT (A B: FinInt 32): SSAEnv arith := SSAEnv.One [
 ]
 
 theorem equivalent (A B: FinInt 32):
-    (run ⟦LHS⟧ (INPUT A B) |>.snd.get "r" .i32) =
-    (run ⟦RHS⟧ (INPUT A B) |>.snd.get "r" .i32) := by
+  semanticPostCondition₂
+    (run ⟦LHS⟧ (INPUT A B))
+    (run ⟦RHS⟧ (INPUT A B))
+  fun _ env₁ _ env₂ =>
+    env₁.get "r" .i32 = env₂.get "r" .i32 := by
   simp [LHS, RHS, INPUT]
-  simp [run, denoteBB, denoteBBStmt, denoteBBStmts, denoteOp]; dsimp_itree
-  simp [interpUB']; dsimp_itree
-  simp [interpSSA', Fitree.interpState, SSAEnvE.handle, SSAEnv.get]; dsimp_itree
-  repeat (simp [SSAEnv.get]; dsimp_itree)
+  simp [run, denoteBB, denoteBBStmt, denoteBBStmts, denoteOp]; simp_itree
   apply FinInt.add_xor_and
 end th8
 
@@ -704,15 +733,14 @@ def INPUT (B: FinInt 1) (C: FinInt 32): SSAEnv arith := SSAEnv.One [
 ]
 
 theorem equivalent (B: FinInt 1) (C: FinInt 32):
-    (run ⟦LHS⟧ (INPUT B C) |>.snd.get "r" .i32) =
-    (run ⟦RHS⟧ (INPUT B C) |>.snd.get "r" .i32) := by
+  semanticPostCondition₂
+    (run ⟦LHS⟧ (INPUT B C))
+    (run ⟦RHS⟧ (INPUT B C))
+  fun _ env₁ _ env₂ =>
+    env₁.get "r" .i32 = env₂.get "r" .i32 := by
   simp [LHS, RHS, INPUT]
-  simp [run, denoteBB, denoteBBStmt, denoteBBStmts, denoteOp]; dsimp_itree
-  simp [Semantics.semantics_op, arith_semantics_op, AttrDict.find, List.find?,
-        AttrEntry.key, AttrEntry.value]; dsimp_itree
-  simp [interpUB']; dsimp_itree
-  simp [interpSSA', Fitree.interpState, SSAEnvE.handle, SSAEnv.get]; dsimp_itree
-  repeat (simp [SSAEnv.get]; dsimp_itree)
+  simp [run, denoteBB, denoteBBStmts, denoteBBStmt, denoteOp]; simp_itree
+  simp [Semantics.semantics_op, arith_semantics_op]; simp_itree
   apply FinInt.add_bool_eq_select
 end th9
 
@@ -754,8 +782,11 @@ def INPUT (A B C: FinInt 32): SSAEnv arith := SSAEnv.One [
 ]
 
 theorem equivalent (A B C: FinInt 32):
-    (run ⟦LHS⟧ (INPUT A B C) |>.snd.get "r" .i32) =
-    (run ⟦RHS⟧ (INPUT A B C) |>.snd.get "r" .i32) := by
+  semanticPostCondition₂
+    (run ⟦LHS⟧ (INPUT A B C))
+    (run ⟦RHS⟧ (INPUT A B C))
+  fun _ env₁ _ env₂ =>
+    env₁.get "r" .i32 = env₂.get "r" .i32 := by
   simp [INPUT, LHS, RHS, run, denoteBB, denoteBBStmts]
   rw [ops.constant.sem]
   rw [ops.negi.sem]
@@ -766,9 +797,7 @@ theorem equivalent (A B C: FinInt 32):
   rw [ops.ori.sem]
   rw [ops.xori.sem]
   rw [ops.andi.sem]
-  simp [interpUB']; dsimp_itree
-  simp [interpSSA', Fitree.interpState, SSAEnvE.handle]; dsimp_itree
-  repeat (simp [SSAEnv.get, SSAEnv.set]; simp_itree)
+  simp [interpSSA', Fitree.interpState, SSAEnvE.handle]; simp_itree
   apply FinInt.and_not_and_not
 end th10
 
@@ -809,8 +838,11 @@ def INPUT (A B: FinInt 32): SSAEnv arith := SSAEnv.One [
 ]
 
 theorem equivalent (A B: FinInt 32):
-    (run ⟦LHS⟧ (INPUT A B) |>.snd.get "r" .i32) =
-    (run ⟦RHS⟧ (INPUT A B) |>.snd.get "r" .i32) := by
+  semanticPostCondition₂
+    (run ⟦LHS⟧ (INPUT A B))
+    (run ⟦RHS⟧ (INPUT A B))
+  fun _ env₁ _ env₂ =>
+    env₁.get "r" .i32 = env₂.get "r" .i32 := by
   simp [INPUT, LHS, RHS, run, denoteBB, denoteBBStmts]
   rw [ops.constant.sem]
   rw [ops.negi.sem]
@@ -820,9 +852,7 @@ theorem equivalent (A B: FinInt 32):
   rw [ops.ori.sem]
   rw [ops.xori.sem]
   rw [ops.xori.sem]
-  simp [interpUB']; dsimp_itree
-  simp [interpSSA', Fitree.interpState, SSAEnvE.handle]; dsimp_itree
-  repeat (simp [SSAEnv.get, SSAEnv.set]; simp_itree)
+  simp [interpSSA', Fitree.interpState, SSAEnvE.handle]; simp_itree
   apply FinInt.and_or_not_or
 end th11
 
@@ -857,12 +887,12 @@ def INPUT (X C₁ C₂: FinInt 32): SSAEnv arith := SSAEnv.One [
 ]
 
 theorem equivalent (X C₁ C₂: FinInt 32):
-    (run ⟦LHS⟧ (INPUT X C₁ C₂) |>.snd.get "r" .i32) =
-    (run ⟦RHS⟧ (INPUT X C₁ C₂) |>.snd.get "r" .i32) := by
+  semanticPostCondition₂
+    (run ⟦LHS⟧ (INPUT X C₁ C₂))
+    (run ⟦RHS⟧ (INPUT X C₁ C₂))
+  fun _ env₁ _ env₂ =>
+    env₁.get "r" .i32 = env₂.get "r" .i32 := by
   simp [LHS, RHS, INPUT]
   simp [run, denoteBB, denoteBBStmts, denoteBBStmt, denoteOp]; simp_itree
-  simp [interpUB']; simp_itree
-  simp [interpSSA', Fitree.interpState, SSAEnvE.handle, SSAEnv.get]; simp_itree
-  repeat (simp [SSAEnv.get]; simp_itree)
   apply FinInt.xor_and
 end th12
